Traat/criticalpairs.lean
@@ -1,0 +1,75 @@
+import Traat.chapter3
+
+section Position
+
+#print Option
+
+inductive Move where | left | right
+
+open Move Term
+
+-- A position in a term is just a sequence of moves to a "head" position.
+abbrev Position := List Move
+
+def Position.valid (p : Position) (t : Term) : Bool :=
+  match p, t with
+  | [], _ => true
+  | left::ps, t₁ @@ _ => Position.valid ps t₁
+  | right::ps, _ @@ t₂ => Position.valid ps t₂
+  | _::_, _ => false
+
+def Position.get (p : Position) (t : Term) (h : p.valid t) : Term :=
+  match p, t with
+  | [], _ => t
+  | left::ps, t₁ @@ _ => Position.get ps t₁ h
+  | right::ps, _ @@ t₂ => Position.get ps t₂ h
+  | _::_, _ => t
+
+#eval ("f" @@ var "x" @@ var "y")
+
+#eval let p : Position := [left, left]
+  p.get ("f" @@ var "x" @@ var "y") (refl true)
+
+
+def Position.get? (p : Position) (t : Term) : Option Term :=
+  match p, t with
+  | [], _ => t
+  | left::ps, t₁ @@ _ => Position.get? ps t₁
+  | right::ps, _ @@ t₂ => Position.get? ps t₂
+  | _::_, _ => none
+
+abbrev Position.head : Position := []
+
+@[simp, grind .]
+lemma varValidHead (h : p.valid (var x)) : p = Position.head := by
+  revert h; induction p <;> grind [Position.valid]
+
+@[simp, grind .]
+lemma funcValidHead (h : p.valid (func x)) : p = Position.head := by
+  revert h; induction p <;> grind [Position.valid]
+
+
+lemma Position.validSubst (p : Position) (t : Term) (σ : Subst)
+  (h : p.valid t)
+  : p.valid <| t.apply σ := by
+  match p, t with
+  | [], _ => simp [valid]
+  | left::ps, t₁ @@ t₂ =>
+    simp [apply, valid]; apply Position.validSubst
+    . simp [valid] at h; trivial
+  | right::ps, t₁ @@ t₂ =>
+    simp [apply, valid]; apply Position.validSubst
+    . simp [valid] at h; trivial
+  | _::_, var _ => simp [valid] at h
+  | _::_, func _ => simp [valid] at h
+
+lemma validAppend {p₁ p₂ : Position} (h : (p₁++p₂).valid t)
+  : p₁.valid t := by sorry
+
+lemma validAppendTail {p₁ p₂ : Position} (h : (p₁++p₂).valid t)
+  : p₂.valid <| p₁.get t (validAppend h) := by sorry
+
+lemma getAppend {p₁ p₂ : Position} (h : (p₁++p₂).valid t)
+  : (p₁ ++ p₂).get t h = p₂.get (p₁.get t <| validAppend h) (validAppendTail h) := by sorry
+
+end Position
